Maybe I should'nt insist on an equivalence for val...
...but simply use equality.

theories/Infra/Option.v
@@ -1,4 +1,4 @@
-Require Import List.
+Require Import List Coq.Classes.Equivalence Containers.OrderedTypeEx.
 
 (** Cast option in the framework of Monad. The code in this file is taken from CompCert. *)
 
@@ -7,85 +7,113 @@ Notation "⎣⎦" := (None) (at level 0).
 
 Set Implicit Arguments.
 
-Definition bind (A B : Type) (f : option A) (g : A -> option B) : option B :=
-  match f with
+Definition bind (A B : Type) (g : A -> option B) (x : option A) : option B :=
+  match x with
     | Some a => g a
     | None   => None
   end.
 
 Extraction Inline bind.
 
-Notation "'mdo' X <- A ; B" := (bind A (fun X => B))
+Notation "'mdo' X <- A ; B" := (bind (fun X => B) A)
  (at level 200, X ident, A at level 100, B at level 200).
 
-Lemma bind_inversion (A B : Type) (f : option A) (g : A -> option B) (y : B) :
-  bind f g = Some y -> exists x, f = Some x /\ g x = Some y.
+Lemma bind_inversion_Some (A B : Type) (f : option A) (g : A -> option B) (y : B) :
+  bind g f = Some y -> { x : A | f = Some x /\ g x = Some y }.
 Proof.
   destruct f. firstorder. discriminate.
 Qed.
 
-Lemma bind_inversion' (A B : Type) (f : option A) (g : A -> option B) (y : B) :
-  bind f g = Some y -> { x : A | f = Some x /\ g x = Some y }.
-Proof.
-  destruct f. firstorder. discriminate.
-Qed.
-
-(** * Reasoning over monadic computations *)
-
-(** The [monadInv H] tactic below simplifies hypotheses of the form
-<<
-        H: (do x <- a; b) = OK res
->>
-    By definition of the bind operation, both computations [a] and
-    [b] must succeed for their composition to succeed.  The tactic
-    therefore generates the following hypotheses:
-
-         x: ...
-        H1: a = OK x
-        H2: b x = OK res
-*)
-
-
-Lemma bind_inversion'' {A B : Type} (f : option A) (g : A -> option B) :
-  bind f g = None -> f = None \/ exists x, f = Some x /\ g x = None.
+Lemma bind_inversion_None {A B : Type} (f : option A) (g : A -> option B) :
+  bind g f = None -> f = None \/ exists x, f = Some x /\ g x = None.
 Proof.
   destruct f; firstorder.
 Qed.
 
+Lemma bind_inversion_Some_equiv (A B : Type) `{Equivalence B}
+      (f : option A) (g : A -> option B) (y : B) :
+  bind g f === Some y -> { x : A | f = Some x /\ g x === Some y }.
+Proof.
+  intros.
+  destruct f; simpl in *. firstorder.
+  intros; exfalso. inversion H0.
+Qed.
+
+Lemma bind_inversion_None_equiv {A B : Type} `{Equivalence B} (f : option A) (g : A -> option B) :
+  bind g f === None -> f = None \/ exists x, f = Some x /\ g x = None.
+Proof.
+  destruct f; firstorder.
+  inversion H0; subst; eauto.
+Qed.
+
+Lemma option_eq_inv X R (x:X) x'
+  : @option_eq _ R (Some x) (Some x') -> R x x'.
+Proof.
+  inversion 1; eauto.
+Qed.
+
 Ltac monad_simpl :=
   match goal with
-    | [ H: ?F = _ |- appcontext [bind ?F ?G = _] ] => rewrite H; simpl
-  end.
-
-Ltac monad_inv1 H :=
-  match type of H with
-  | (Some _ = Some _) =>
-      inversion H; clear H; try subst
-  | (None   = Some _) =>
-      discriminate
-  | (bind ?F ?G = Some ?X) =>
-      let x   := fresh "x"  in (
-      let EQ1 := fresh "EQ" in (
-      let EQ2 := fresh "EQ" in (
-        destruct (bind_inversion' F G H) as [x [EQ1 EQ2]];
-        clear H;
-        try (monad_inv1 EQ2))))
-  | (bind ?F ?G = None) =>
-    let x   := fresh "x"  in
-    let EQ1 := fresh "EQ" in
-    let EQ2 := fresh "EQ" in
-    destruct (bind_inversion'' F G H) as [|[x [EQ1 EQ2]]];
-      clear H;
-      try (monad_inv1 EQ2)
+    | [ H: ?F = _ |- context [bind ?F ?G = _] ] => rewrite H; simpl
   end.
 
 Ltac monad_inv H :=
   match type of H with
-  | (Some _ = Some _) => monad_inv1 H
-  | (None   = Some _) => monad_inv1 H
-  | (Some _ = None) => monad_inv1 H
-  | (bind ?F ?G = Some ?X) => monad_inv1 H
-  | (bind ?F ?G = None) => monad_inv1 H
-  | (@eq _ (@bind _ _ _ _ _ ?G) (?X)) =>
-    let X := fresh in remember G as X; simpl in H; subst X; monad_inv1 H
+  | (Some _ = Some _) =>
+    inversion H; clear H; try subst
+  | (None   = Some _) =>
+    inversion H
+  | (Some _ = None) =>
+    inversion H
+  | (Some _ === Some _) =>
+    eapply option_eq_inv in H; try subst
+  | (None === Some _) =>
+    exfalso; inversion H
+  | (Some _ === None) =>
+    exfalso; inversion H
+  | (bind ?F ?G = Some ?X) =>
+    let x   := fresh "x"  in
+    let EQ1 := fresh "EQ" in
+    let EQ2 := fresh "EQ" in
+    destruct (bind_inversion_Some G F H) as [x [EQ1 EQ2]];
+    clear H;
+    try (monad_inv EQ2)
+  | (bind ?F ?G = None) =>
+    let x   := fresh "x"  in
+    let EQ1 := fresh "EQ" in
+    let EQ2 := fresh "EQ" in
+    destruct (bind_inversion_None G F H) as [|[x [EQ1 EQ2]]];
+    clear H;
+    try (monad_inv EQ2)
+  | (bind ?F ?G === Some ?X) =>
+    let x   := fresh "x"  in
+    let EQ1 := fresh "EQ" in
+    let EQ2 := fresh "EQ" in
+    destruct (bind_inversion_Some_equiv G F H) as [x [EQ1 EQ2]];
+    clear H;
+    try (monad_inv EQ2)
+  | (bind ?F ?G === None) =>
+    let x   := fresh "x"  in
+    let EQ1 := fresh "EQ" in
+    let EQ2 := fresh "EQ" in
+    destruct (bind_inversion_None_equiv G F H) as [|[x [EQ1 EQ2]]];
+    clear H;
+    try (monad_inv EQ2)
   end.
+
+Inductive option_R_Some (A B : Type) (eqA : A -> B -> Prop)
+: option A -> option B -> Prop :=
+| Option_R_Some a b : eqA a b -> option_R_Some eqA ⎣a⎦ ⎣b⎦.
+
+
+Lemma option_R_Some_refl A R `{Reflexive A R} : forall x, option_R_Some R ⎣x⎦ ⎣x⎦.
+intros; eauto using option_R_Some.
+Qed.
+
+Instance option_R_Some_sym A R `{Symmetric A R} : Symmetric (option_R_Some R).
+hnf; intros ? [] []; eauto using option_R_Some.
+Qed.
+
+Instance option_R_trans A R `{Transitive A R} : Transitive (option_R_Some R).
+hnf; intros. inversion H0; subst; inversion H1; subst; econstructor; eauto.
+Qed.
