theories/Isa/Val.v
@@ -14,38 +14,11 @@ Instance inst_val_defaulted : Defaulted val := {
   default_el := default_val
 }.
 
-(** Default value for true = 1 = 2^1 , false = 0 = 2^0 **)
-Definition val_true := Int.one.
-Definition val_false := Int.zero.
-Lemma val_true_false_neq
-  : val_true <> val_false.
-Proof.
-  eapply Int.one_not_zero.
-Qed.
-
 Definition val_zero : val := Int.zero.
 
 Instance inst_eq_dec_val : EqDec val eq.
 hnf; intros. eapply Int.eq_dec.
 Defined.
-
-(** ** There must be an injection into the booleans *)
-Definition val2bool (v: val) : bool := if [ v = val_zero ] then false else true.
-
-Lemma val2bool_true
-: val2bool val_true = true.
-Proof.
-  unfold val2bool.
-  cases; eauto.
-  exfalso; eauto using val_true_false_neq.
-Qed.
-
-Lemma val2bool_false
-: val2bool val_false = false.
-Proof.
-  unfold val2bool.
-  cases; eauto.
-Qed.
 
 Inductive binop : Type :=
 | BinOpAdd
@@ -60,23 +33,6 @@ Proof.
   decide equality.
 Qed.
 
-Definition option_lift1 A B (f:A -> B) := fun x => Some (f x).
-Definition option_lift2 A B C (f:A -> B -> C) := fun x y => Some (f x y).
-Definition bool2val (b:bool) :=
-  match b with
-  | true => val_true
-  | false => val_false
-  end.
-
-Definition binop_eval (o:binop) :=
-  match o with
-      | BinOpAdd => option_lift2 Int.add
-      | BinOpSub => option_lift2 Int.sub
-      | BinOpMul => option_lift2 Int.mul
-      | BinOpDiv => option_lift2 Int.divs
-      | BinOpEq => option_lift2 (fun x y => bool2val(Int.eq x y))
-    end.
-
 Inductive unop : Type :=
 | UnOpToBool
 | UnOpNeg.
@@ -86,12 +42,6 @@ Proof.
   hnf; intros. change ({x = y} + {x <> y}).
   decide equality.
 Qed.
-
-Definition unop_eval (o:unop) :=
-  match o with
-  | UnOpToBool => option_lift1 (fun a => bool2val(val2bool a))
-  | UnOpNeg => option_lift1 Int.notbool
-  end.
 
 Declare ML Module "containers_plugin".
 Generate OrderedType unop.
@@ -136,6 +86,28 @@ Proof.
   econstructor; eauto with typeclass_instances.
 Qed.
 
+Definition int_eq x y := Int.intval x = Int.intval y.
+
+Instance Reflexive_eq_int' : Reflexive int_eq.
+Proof.
+  hnf; intros. hnf. reflexivity.
+Qed.
+
+Instance Symmetric_eq_int' : Symmetric int_eq.
+Proof.
+  unfold int_eq. hnf; intros. symmetry; eauto.
+Qed.
+
+Instance Transitive_eq_int' : Transitive int_eq.
+Proof.
+  unfold int_eq. hnf; intros. etransitivity; eauto.
+Qed.
+
+Instance Equivalence_eq_int' : Equivalence int_eq.
+Proof.
+  econstructor; eauto with typeclass_instances.
+Qed.
+
 Instance Transitive_lt_int : Transitive Int.ltu.
 Proof.
   hnf. unfold Int.ltu. intros ? ? ? A B.
@@ -154,15 +126,13 @@ Proof.
 Qed.
 
 Instance int_eq_eq_lt
-  : Proper (Int.eq ==> Int.eq ==> eq) Int.ltu.
+  : Proper (int_eq ==> int_eq ==> eq) Int.ltu.
 Proof.
-  unfold Proper, respectful; intros.
-  pose proof (Int.eq_spec x y).
-  pose proof (Int.eq_spec x0 y0).
-  cases in H1. cases in H2. subst. eauto.
+  unfold Proper, respectful, Int.ltu, Int.unsigned, int_eq; intros.
+  rewrite H, H0. eauto.
 Qed.
 
-Instance StrictOrder_lt_int : StrictOrder Int.ltu Int.eq.
+Instance StrictOrder_lt_int : StrictOrder Int.ltu int_eq.
 Proof.
   econstructor; eauto with typeclass_instances.
   - intros ? ? LE EQ.
@@ -175,40 +145,159 @@ Definition int_compare (x y : int) : Datatypes.comparison :=
 
 Unset Printing Records.
 
-Require ProofIrrelevance.
-
 Lemma compare_spec_int x y
-  : compare_spec Int.eq Int.ltu x y (int_compare x y).
+  : compare_spec int_eq Int.ltu x y (int_compare x y).
 Proof.
   pose proof (Z.compare_spec (Int.intval x) (Int.intval y)).
   case_eq (int_compare x y); intros EQ; econstructor; unfold int_compare in EQ;
-    rewrite EQ in H; inv H.
-  - pose proof (Int.eq_spec x y).
-    hnf. cases; eauto. eapply H1.
-    destruct x,y; simpl in *.
-    subst. assert (intrange = intrange0) by eapply ProofIrrelevance.proof_irrelevance.
-    subst; eauto.
+    rewrite EQ in H; inv H; eauto.
   - hnf. unfold Int.ltu.
     rewrite Coqlib.zlt_true; eauto.
   - hnf. unfold Int.ltu.
     rewrite Coqlib.zlt_true; eauto.
 Qed.
+
+Require Import ProofIrrelevance.
 
 Lemma compare_spec_int_eq x y
   : int_compare x y = Eq -> x = y.
 Proof.
   intros.
   pose proof (compare_spec_int x y). rewrite H in H0.
-  inv H0. pose proof (Int.eq_spec x y). cases in H2. eauto.
+  inv H0. destruct x,y; compute in H1; subst.
+  assert (intrange = intrange0).
+  eapply ProofIrrelevance.proof_irrelevance. subst. reflexivity.
 Qed.
+
+Instance int_eq_dec : EqDec val int_eq.
+hnf; intros. destruct x,y.
+eapply Z.eq_dec.
+Defined.
+
+Instance int_eq_dec' x y : Computable (int_eq x y).
+hnf; intros. destruct x,y.
+eapply Z.eq_dec.
+Defined.
+
 
 Instance OrderedType_int : OrderedType int.
 Proof.
-  eapply (Build_OrderedType _ Int.eq Int.ltu); eauto with typeclass_instances.
+  eapply (Build_OrderedType _ int_eq Int.ltu); eauto with typeclass_instances.
   eapply compare_spec_int.
 Defined.
 
 
+
+Definition option_lift1 A B (f:A -> B) := fun x => Some (f x).
+Definition option_lift2 A B C (f:A -> B -> C) := fun x y => Some (f x y).
+
+Definition val_true := Int.one.
+Definition val_false := Int.zero.
+
+Lemma val_true_false_neq
+  : val_true <> val_false.
+Proof.
+  eapply Int.one_not_zero.
+Qed.
+
+Lemma val_true_false_nequiv
+  : val_true =/= val_false.
+Proof.
+  inversion 1.
+Qed.
+
+Definition bool2val (b:bool) :=
+  match b with
+  | true => val_true
+  | false => val_false
+  end.
+
+
+Definition val2bool (v: val) : bool := if [ v === val_zero ] then false else true.
+
+Lemma val2bool_true
+: val2bool val_true = true.
+Proof.
+  unfold val2bool.
+  cases; eauto.
+  exfalso; eauto using val_true_false_nequiv.
+Qed.
+
+Lemma val2bool_false
+: val2bool val_false = false.
+Proof.
+  unfold val2bool.
+  cases; eauto.
+Qed.
+
+
+Definition binop_eval (o:binop) :=
+  match o with
+      | BinOpAdd => option_lift2 Int.add
+      | BinOpSub => option_lift2 Int.sub
+      | BinOpMul => option_lift2 Int.mul
+      | BinOpDiv => fun x y => if [ y === val_zero] then None else (Some (Int.divs x y))
+      | BinOpEq => option_lift2 (fun x y => bool2val(Int.eq x y))
+    end.
+
+Lemma binop_eval_div_zero x y
+  : y === val_zero
+    <-> binop_eval BinOpDiv x y = None.
+Proof.
+  intros; simpl; cases; split; intros; eauto; exfalso; congruence.
+Qed.
+
+Lemma binop_eval_div_nonzero x y
+  : y =/= val_zero
+    -> exists v, binop_eval BinOpDiv x y = Some v.
+Proof.
+  intros; simpl; cases; eauto.
+  exfalso; eauto.
+Qed.
+
+Lemma binop_eval_not_div op x y
+  : op <> BinOpDiv
+    -> exists v, binop_eval op x y = Some v.
+Proof.
+  intros; destruct op; simpl; unfold option_lift2; eauto.
+  congruence.
+Qed.
+
+Definition unop_eval (o:unop) :=
+  match o with
+  | UnOpToBool => option_lift1 (fun a => bool2val(val2bool a))
+  | UnOpNeg => option_lift1 Int.notbool
+  end.
+
+Lemma unop_eval_total op x
+  : exists v, unop_eval op x = Some v.
+Proof.
+  intros; destruct op; simpl; unfold option_lift1; eauto.
+Qed.
+
+Lemma binop_eval_equiv
+  : Proper (eq ==> equiv ==> equiv ==> equiv ) binop_eval.
+Proof.
+  unfold Proper, respectful; intros; subst.
+  destruct y, x0,x1,y0,y1; compute in H0, H1; subst; simpl; unfold option_lift2;
+    try reflexivity.
+Qed.
+
+Lemma unop_eval_equiv
+  : Proper (eq ==> equiv ==> equiv ) unop_eval.
+Proof.
+  unfold Proper, respectful; intros; subst.
+  destruct y, x0,y0; compute in H0; subst; simpl; unfold option_lift1;
+    try reflexivity.
+Qed.
+
+Lemma unop_eval_equiv'
+  : Proper (equiv ==> equiv ==> equiv ) unop_eval.
+Proof.
+  unfold Proper, respectful; intros; subst.
+  destruct x0,y0; inv H; compute in H0; subst; simpl; unfold option_lift1;
+    try reflexivity.
+Qed.
 
 Opaque val.
 Opaque default_val.
