theories/TransVal/SMT.v
@@ -40,6 +40,14 @@ Proof.
   rewrite H; eauto.
 Qed.
 
+Lemma to_partial_to_total (E:onv val) x v
+  : E x === Some v -> to_partial (to_total E) x === Some v.
+Proof.
+  intros.
+  unfold to_partial, to_total. cases; eauto.
+  inv H.
+Qed.
+
 (** Define what uninterpreted function symbols are **)
 Definition pred := lab (*arglst -> bool*).
 
@@ -146,31 +154,96 @@ intros.
 specialize (H F E). assumption.
 Qed.
 
-Lemma exp_eval_partial_total E e v
- : exp_eval E e = Some v ->
-   exp_eval (to_partial (to_total E)) e = Some v.
+Instance bind_equiv (A B : Type) `{Equivalence A} `{Equivalence B}
+         (f:A -> option B) `{Proper _ (Equivalence.equiv ==> Equivalence.equiv) f}
+  : Proper (Equivalence.equiv ==> Equivalence.equiv) (@bind A B f).
 Proof.
-  intros. general induction e; simpl in * |- *; eauto.
-  - unfold to_partial, to_total; simpl. rewrite H; eauto.
-  - monad_inv H; simpl. rewrite EQ. erewrite IHe; eauto.
-  - monad_inv H; simpl.
-    erewrite IHe1; eauto. erewrite IHe2; eauto.
-    rewrite EQ, EQ1; simpl; eauto.
+  unfold Proper, respectful; intros; subst.
+  inv H2; simpl; eauto.
+Qed.
+
+Instance bind_binop_eval1 op v
+  : Proper (Equivalence.equiv ==> Equivalence.equiv)
+           (fun v' => bind (binop_eval op v') v).
+Proof.
+  hnf; intros. destruct v; simpl; eauto.
+  eapply binop_eval_equiv; eauto.
+Qed.
+
+Instance bind_binop_eval2 op v
+  : Proper (Equivalence.equiv ==> Equivalence.equiv)
+           (fun v' : Integers.Int.int => binop_eval op v v').
+Proof.
+  hnf; intros. destruct v; simpl; eauto.
+  eapply binop_eval_equiv; eauto.
+Qed.
+
+(*
+this doesn't help, setoid rewrite needs the instance above
+Instance test (A:Type) v `{Equivalence A}
+         (f : A -> A -> ؟ A)
+         `{Proper _ (Equivalence.equiv ==> Equivalence.equiv ==> Equivalence.equiv) f}
+  : Proper (Equivalence.equiv ==> Equivalence.equiv)
+           (fun v1 : A => bind (f v1) v).
+Proof.
+  hnf; intros. destruct v; simpl; eauto.
+  eapply H0; eauto.
+Qed.
+*)
+
+
+Lemma eq_equiv X (x y:X) `{Equivalence X}
+  : x = y -> x === y.
+Proof.
+  intros; subst; eauto.
+Qed.
+
+Hint Immediate eq_equiv.
+
+Lemma exp_eval_partial_total E e v
+ : exp_eval E e === Some v ->
+   exp_eval (to_partial (to_total E)) e === Some v.
+Proof.
+  intros.
+  general induction e; simpl in * |- *; eauto.
+  - erewrite to_partial_to_total; eauto.
+  - monad_inv H; simpl; eauto.
+    exploit IHe; eauto.
+    rewrite bind_equiv; eauto; simpl. eauto.
+    eapply unop_eval_equiv; eauto.
+  - intros.
+    monad_inv H; simpl.
+    rewrite IHe1; eauto; simpl.
+    rewrite IHe2; eauto.
+Qed.
+
+Instance bind_list A B (f:A -> option (list B)) `{Equivalence A} `{Equivalence B} a
+  : Proper (Equivalence.equiv ==> option_eq (list_eq R0))
+           (fun v  => mdo vl0 <- f a; ⎣ v :: vl0 ⎦).
+Proof.
+  unfold Proper, respectful; intros.
+  destruct (f a); simpl; eauto.
+  econstructor; econstructor; eauto. reflexivity.
+  econstructor.
 Qed.
 
 (** Next 2 Lemmata belong to Lemma 4 in subsection 3.4 in the thesis
 They prove that evaluation without a total environment is equal
 to evaluation under a total environment **)
 Lemma exp_eval_partial_total_list E el vl
-:  omap (exp_eval E) el = Some vl
--> omap (exp_eval (to_partial (to_total  E))) el = Some vl.
+:  omap (exp_eval E) el === Some vl
+-> omap (exp_eval (to_partial (to_total  E))) el === Some vl.
 
 Proof.
   intros. general induction el; eauto using exp_eval_partial_total.
-  - simpl in H. monad_inv H.
-    specialize (IHel E x0 EQ1).
-    rewrite EQ. rewrite EQ1.
-    simpl; erewrite exp_eval_partial_total; eauto.
+  - simpl in H. monad_inv H. simpl.
+    erewrite (exp_eval_partial_total _ _ (eq_equiv EQ)); eauto.
+    simpl.
+    exploit IHel; eauto.
+    rewrite bind_equiv; [ | | eapply H ]. eauto; simpl.
+    econstructor; eauto.
+    eapply bind_list.
+
     rewrite IHel; eauto.
 Qed.
 
